Documentation of CVIR (understanding purpose)

examples/Imp2Vir/CvirCombinators.v
@@ -24,8 +24,9 @@ Record cvir (n_in n_out : nat) : Type := {
      (v_out : Vec.t raw_id n_out)
      (v_int : Vec.t raw_id n_int),
      list (block typ);
-}.
+                                      }.
 
+ (* Given a blocks, returns the corresponding CVIR *)
 Definition mk_cvir
   {n_in n_out n_int : nat}
   (blocks : forall
@@ -43,6 +44,11 @@ Definition mk_cvir
 Arguments n_int {_} {_}.
 Arguments blocks {_} {_}.
 
+
+(** Basic CVIR *)
+
+(* Take a code (ie. list of instructions) and create a simple CVIR with 1 input
+and 1 output (inconditional branch) *)
 Definition block_cvir (c : code typ) : cvir 1 1 :=
   mk_cvir (fun
     (vi : Vec.t raw_id 1)
@@ -51,6 +57,8 @@ Definition block_cvir (c : code typ) : cvir 1 1 :=
     => [mk_block (Vec.hd vi) List.nil c (TERM_Br_1 (hd vo)) None]
   ).
 
+(* Take a code (ie. list of instructions) and an expression, and create a simple
+ CVIR with 1 input and 2 outputs (conditional branch on e) *)
 Definition branch_cvir (c : code typ) (e : texp typ) : cvir 1 2 :=
   mk_cvir (fun
     (vi : Vec.t raw_id 1)
@@ -59,27 +67,37 @@ Definition branch_cvir (c : code typ) (e : texp typ) : cvir 1 2 :=
     => [mk_block (Vec.hd vi) (List.nil) c (TERM_Br e (Vec.hd vo) (Vec.hd (Vec.tl vo))) None]
   ).
 
+(* Take a code (ie. list of instructions) and an expression, and create a simple
+ CVIR with 1 input and no output (block returns e) *)
 Definition ret_cvir (c : code typ) (e : texp typ) : cvir 1 0 :=
   mk_cvir (fun vi vo (vt : Vec.t raw_id 0) =>
     [mk_block (Vec.hd vi) List.nil c (TERM_Ret e) None]
   ).
 
+(* Take a code (ie. list of instructions) and an expression, and create a simple
+ CVIR with 1 input and no output (block returns void) *)
 Definition ret_void_cvir (c : code typ) : cvir 1 0 :=
   mk_cvir (fun vi vo (vt : Vec.t raw_id 0) =>
     [mk_block (Vec.hd vi) List.nil c (TERM_Ret_void) None]
   ).
 
+(** Combinators over CVIR *)
+
+
+(* Taking 2 cvir as input, create a new cvir concanating inputs and ouputs
+// similar to app_asm in itree tutorial *)
 Definition merge_cvir
-  {ni1 no1 ni2 no2 : nat}
-  (b1: cvir ni1 no1)
-  (b2: cvir ni2 no2) :
+           {ni1 no1 ni2 no2 : nat}
+           (b1: cvir ni1 no1)
+           (b2: cvir ni2 no2) :
   cvir (ni1+ni2) (no1+no2) :=
-    mk_cvir (fun vi vo vt =>
-      let '(li,ri) := Vec.splitat ni1 vi in
-      let '(lo,ro) := Vec.splitat no1 vo in
-      let '(lt,rt) := Vec.splitat (n_int b1) vt in
-      (blocks b1 li lo lt) ++ (blocks b2 ri ro rt)
-    ).
+  mk_cvir (fun vi vo vt =>
+    let '(li,ri) := Vec.splitat ni1 vi in
+    let '(lo,ro) := Vec.splitat no1 vo in
+    let '(lt,rt) := Vec.splitat (n_int b1) vt in
+    (blocks b1 li lo lt) ++ (blocks b2 ri ro rt)).
+
+(* Reordering of the vectors *)
 
 Definition sym_i_cvir {ni1 ni2 ni3 no : nat} (b : cvir (ni1 + (ni2 + ni3)) no) :
   cvir (ni1 + (ni3 + ni2)) no :=
@@ -101,8 +119,10 @@ Definition cast_i_cvir {ni ni' no : nat} (b : cvir ni no) (H : ni = ni') : cvir 
 Definition cast_o_cvir {ni no no' : nat} (b : cvir ni no) (H : no = no') : cvir ni no' :=
   mk_cvir (fun vi vo (vt : Vec.t raw_id (n_int b)) =>
     blocks b vi (Vec.cast vo (eq_sym H)) vt
-  ).
+          ).
 
+(* NOTE (vi=(0,1,2,3,4,5), i = 4) => (vi->(4,0,1,2,3,5)) *)
+(* Bring the i-th input at the head of the input vector *)
 Program Definition focus_input_cvir {ni no : nat} (b : cvir ni no) (i : Fin.fin ni) : cvir ni no :=
   let b := cast_i_cvir b (_ : ni = proj1_sig i + (1 + (ni - proj1_sig i - 1)))%nat in
   let b := sym_i_cvir b in
@@ -120,9 +140,11 @@ Next Obligation.
   lia.
 Defined.
 Next Obligation.
-  destruct ni ; [ destruct i |] ; lia.
+  destruct ni; destruct i ; lia.
 Defined.
 
+
+(* Bring the i-th output at the head of the output vector *)
 Program Definition focus_output_cvir {ni no : nat} (b : cvir ni no) (o : Fin.fin no) : cvir ni no :=
   let b := cast_o_cvir b (_ : no = proj1_sig o + (1 + (no - proj1_sig o - 1)))%nat in
   let b := sym_o_cvir b in
@@ -143,54 +165,65 @@ Next Obligation.
   destruct no ; [ destruct o |] ; lia.
 Defined.
 
+(* Connect the fist input and the first output of a CVIR and internalize them *)
 Definition loop_cvir {ni no : nat} (b : cvir (S ni) (S no)) : cvir ni no :=
   mk_cvir (fun vi vo vt =>
     let '(newint,vt) := Vec.uncons vt in
     (blocks b) (newint :: vi)%vec (newint :: vo)%vec vt
   ).
 
+(* wrapper for loop_cvir *)
 Definition loop_cvir' {ni no ni' no' : nat} (b : cvir ni no)
   (Heqi : ni = S ni') (Heqo : no = S no') :
   cvir ni' no' :=
   loop_cvir (cast_o_cvir (cast_i_cvir b Heqi) Heqo).
 
+
+(* Connect the first input of b2 to the first output of b1 *)
 Program Definition seq_cvir {ni1 no1 ni2 no2 : nat}
   (b1 : cvir ni1 (S no1))
   (b2: cvir (S ni2) no2) :
   cvir (ni1+ni2) (no1+no2) :=
-    let b := merge_cvir b1 b2 in
-    let b := focus_input_cvir b (fi' ni1) in
-    loop_cvir' b _ _.
+  (* firstly, merge b1 and b2 *)
+  let b := merge_cvir b1 b2 in
+  (* bring the first output of b2 at the first place of b *)
+  let b := focus_input_cvir b (fi' ni1) in
+  (* connect the first input of b (ie. 1st input of b2)
+     to the first output of b (ie. 1st ouput of b1) *)
+  loop_cvir' b _ _.
 Next Obligation.
   apply Nat.lt_add_pos_r.
   apply Nat.lt_0_succ.
 Defined.
 
+(* Connect the first output of b to its first input, and internalize the only
+the ouput *)
 Definition loop_cvir_open {ni no : nat} (b : cvir (S ni) (S no)) : cvir (S ni) no :=
   mk_cvir (fun vi vo vt =>
-    (blocks b) vi (hd vi :: vo)%vec vt
-  ).
+    (blocks b) vi (hd vi :: vo)%vec vt).
 
+
+(* Merge the first output with the second one *)
 Definition join_cvir {ni no : nat} (b : cvir ni (S (S no))) : cvir ni (S no) :=
   mk_cvir (fun vi vo vt =>
     let o := Vec.hd vo in
-    (blocks b) vi (o :: vo)%vec vt
-  ).
+    (blocks b) vi (o :: vo)%vec vt).
 
+(* Remove the inputs of a cvir (without output)... Is that useful ? *)
 Definition close_cvir {ni} (b : cvir ni 0) : cvir 0 0 :=
   mk_cvir (fun vi vo vt =>
     let '(vi,vt) := Vec.splitat ni vt in
-    (blocks b) vi vo vt
-  ).
+    (blocks b) vi vo vt).
 
-(*Definition cond_cvir {ni1 no1 ni2 no2 : nat}
+(*
+Definition cond_cvir {ni1 no1 ni2 no2 : nat}
   (b1 : cvir (S ni1) (S no1)) (b2: cvir (S ni2) (S no2)) (e : texp typ) :
   cvir (ni1+ni2) (no1+no2) :=
     let cond_ir := branch_cvir [] e in
     let branchs_ir := join_cvir b1 b2 in
     seq_cvir cond_ir branchs_ir
     join_cvir (cast_o_cvir (seq_cvir (seq_cvir cond_ir b1) b2) _).
-*)
+ *)
 
 Definition fnbody := (block typ * list (block typ))%type.
 Definition program := toplevel_entity typ fnbody.
