examples/Imp2Vir/README.md
@@ -1,0 +1,13 @@
+ [CompileExpr](./CompileExpr.v): Compile Imp expressions into VIR expression
+ [CvirCombinators](./CvirCombinators.v): Define CVIR and basic combinators over CVIR 
+ [CvirCombinatorsWF](./CvirCombinatorsWF.v): Well-Formness properties over CVIR
+ [Fin](./Fin.v): Theory over Finite types as a categorical embedding (imported from itree tutorial)
+ [Imp](./Imp.v): Syntax, Semantic and Interpretation of Imp (imported from itree tutorial)
+ [Imp2Cvir](./Imp2Cvir.v): Compiler from Imp to CVir
+ [Relabel](./Relabel.v): Relabeling theory 
+ [Semantics](./Semantics.v): Denotation of a CVir construct
+ [Sir](./Sir.v):(Structured IR) Ancestor of CVIR (depreciated)
+ [Unique](./Unique.v): Utilities (imported from itree tutorial)
+ [Utils](./Utils.v): Utilities over standard librairy, extlib and vellvm
+ [Utils_tutorial](./Utils_tutorial.v): Utilities (imported from itree tutorial)
+ [Vec](./Vec.v): Definition and theory of vectors
